max_certified_epoch

steel/Zeta.Steel.AggregateEpochHashes.fsti
@@ -55,48 +55,48 @@ let epoch_tid_bitmaps =
     epoch_id_hash
     (fun i -> A.pts_to)
 
-let is_epoch_verified (eid:M.epoch_id) (lve:M.epoch_id) =
-  U32.v lve >= U32.v eid
+let is_epoch_verified (tsm:M.thread_state_model) (eid:M.epoch_id) =
+  U32.v tsm.M.last_verified_epoch >= U32.v eid
 
-[@@erasable]
-let epoch_hash_contributions_t =
-  erased (Seq.lseq epoch_hashes_repr (U32.v n_threads))
-
-let thread_contribs (contribs:epoch_hash_contributions_t) (tid:tid) =
-  Seq.index contribs (U16.v tid)
-
-let upd_thread_contribs (contribs:epoch_hash_contributions_t)
-                        (tid:tid)
-                        (v:_) =
-  Seq.upd contribs (U16.v tid) v
+let all_threads_epoch_hashes =
+  Seq.lseq epoch_hashes_repr (U32.v n_threads)
 
 let aggregate_epoch_hash (e0 e1:M.epoch_hash)
   : M.epoch_hash
   = { hadd = HA.aggregate_hashes e0.hadd e1.hadd;
       hevict = HA.aggregate_hashes e0.hevict e1.hevict}
 
-let aggregate_thread_epoch_hashes (e:M.epoch_id)
-                                  (contribs:epoch_hash_contributions_t)
+let log = Seq.seq log_entry_base
+let all_processed_entries = Seq.lseq log (U32.v n_threads)
+
+let tsm_of_log (mlogs_v:all_processed_entries) (t:tid) =
+  M.verify_model (M.init_thread_state_model t)
+                 (Seq.index mlogs_v (U16.v t))
+
+let thread_contrib_of_log (t:tid) (l:log)
+  : epoch_hashes_repr
+  = let tsm = M.verify_model (M.init_thread_state_model t) l in
+    Zeta.Steel.Util.map_literal
+      (fun (e:M.epoch_id) ->
+         if is_epoch_verified tsm e
+         then Map.sel tsm.epoch_hashes e
+         else M.init_epoch_hash)
+
+let all_threads_epoch_hashes_of_logs (mlogs_v:all_processed_entries)
+  : all_threads_epoch_hashes
+  = Zeta.SeqAux.mapi mlogs_v
+                     (fun tid -> thread_contrib_of_log (U16.uint_to_t tid) (Seq.index mlogs_v tid))
+
+let aggregate_all_threads_epoch_hashes (e:M.epoch_id)
+                                       (mlogs_v:all_processed_entries)
   : M.epoch_hash
   = Zeta.SeqAux.reduce M.init_epoch_hash
                        (fun (s:epoch_hashes_repr) -> aggregate_epoch_hash (Map.sel s e))
-                       contribs
-
-let frame_aggregate_thread_epoch_hashes (e e':M.epoch_id)
-                                        (contribs:epoch_hash_contributions_t)
-                                        (tid:tid)
-                                        (v:M.epoch_hash)
-  : Lemma (requires e <> e')
-          (ensures (
-            let tid = U16.v tid in
-            aggregate_thread_epoch_hashes e contribs ==
-            aggregate_thread_epoch_hashes e (Seq.upd contribs tid (Map.upd (Seq.index contribs tid) e' v))))
-  = admit()
-
+                       (all_threads_epoch_hashes_of_logs mlogs_v)
 
 (* Global monotonic log of entries *)
-let log = Seq.seq log_entry_base
-let all_processed_entries = Seq.lseq log (U32.v n_threads)
+
+
 let map_of_seq (a:all_processed_entries)
   : Map.t tid log
   = map_literal (fun (tid:tid) -> Seq.index a (U16.v tid))
@@ -118,24 +118,13 @@ let committed_tsm_of_logs (mlogs_v:all_processed_entries) (t:tid) =
    M.verify_model (M.init_thread_state_model t)
                   (M.committed_log_entries (log_of_tid mlogs_v t))
 
-let thread_contrib_of_log (t:tid) (l:log)
-  : epoch_hashes_repr
-  = let tsm = M.verify_model (M.init_thread_state_model t) l in
-    Zeta.Steel.Util.map_literal
-      (fun (e:M.epoch_id) ->
-         if is_epoch_verified e tsm.last_verified_epoch
-         then Map.sel tsm.epoch_hashes e
-         else M.init_epoch_hash)
-
-let contribs_of_logs (mlogs_v:all_processed_entries)
-  : epoch_hash_contributions_t
-  = Zeta.SeqAux.mapi mlogs_v
-                     (fun tid -> thread_contrib_of_log (U16.uint_to_t tid) (Seq.index mlogs_v tid))
 
 let all_contributions_are_accurate (global:epoch_hashes_repr)
                                    (mlogs_v:all_processed_entries)
   : prop
-  = forall (e:M.epoch_id). Map.sel global e == aggregate_thread_epoch_hashes e (contribs_of_logs mlogs_v)
+  = forall (e:M.epoch_id). Map.sel global e == aggregate_all_threads_epoch_hashes e mlogs_v
+
+let all_ones = Seq.create (U32.v n_threads) true
 
 let max_certified_epoch_is (global:epoch_hashes_repr)
                            (bitmaps: IArray.repr M.epoch_id tid_bitmap)
@@ -143,78 +132,31 @@ let max_certified_epoch_is (global:epoch_hashes_repr)
   : prop
   = forall (e:M.epoch_id).
        U32.v e <= U32.v max ==>
-       (Map.sel bitmaps e) == Seq.create (U32.v n_threads) true /\
+       (Map.sel bitmaps e) == all_ones /\
        (Map.sel global e).hadd == (Map.sel global e).hevict
 
-let contribs_and_max_ok (global:epoch_hashes_repr)
-                        (bitmaps: IArray.repr M.epoch_id tid_bitmap)
-                        (max:M.epoch_id)
-                        (mlogs_v:all_processed_entries)
- : prop
- = all_contributions_are_accurate global mlogs_v /\
-   max_certified_epoch_is global bitmaps max
 
-let tid_index = i:U16.t { U16.v i <= U32.v n_threads }
+let epoch_is_complete (mlogs_v:all_processed_entries) (e:M.epoch_id)
+  = forall tid. is_epoch_verified (tsm_of_log mlogs_v tid) e
 
-noextract
-let n_threads_16 : tid_index = U16.uint_to_t (U32.v n_threads)
-
-let rec forall_threads_between (from:tid_index)
-                               (to:tid_index { U16.v from <= U16.v to })
-                               (f:tid -> vprop)
-
-  : Tot (vprop)
-        (decreases (U16.v to - U16.v from))
-  = if from = to then emp
-    else f from `star`
-         forall_threads_between U16.(from +^ 1us) to f
-
-let forall_threads (f: tid -> vprop) =
-  forall_threads_between 0us n_threads_16 f
-
-let per_thread_max_and_bitmap (max:M.epoch_id)
-                              (bitmaps: IArray.repr M.epoch_id tid_bitmap)
-                              (tid:tid)
+let per_thread_bitmap_and_max (bitmaps: IArray.repr M.epoch_id tid_bitmap)
+                              (max:M.epoch_id)
                               (all_logs:all_processed_entries)
+                              (tid:tid)
   : prop
   = let tsm = M.verify_model (M.init_thread_state_model tid) (log_of_tid all_logs tid) in
     U32.v max <= U32.v tsm.last_verified_epoch /\ //max can't exceed the verified epoch ctr for tid
     (forall (eid:M.epoch_id).
-      Seq.index (Map.sel bitmaps eid) (U16.v tid) == is_epoch_verified eid tsm.last_verified_epoch)
+      Seq.index (Map.sel bitmaps eid) (U16.v tid) == is_epoch_verified tsm eid)
 
-let per_thread_invariant (max:_)
-                         (bitmaps:_)
-                         (all_logs: all_processed_entries)
-                         ([@@@smt_fallback] tid:tid) =
-    pure (per_thread_max_and_bitmap max bitmaps tid all_logs)
-
-val take_thread (#o:_) (#p:tid -> vprop) (i:tid)
-  : STGhostT unit o
-    (forall_threads p)
-    (fun _ -> p i `star`
-         forall_threads_between 0us i p `star`
-         forall_threads_between U16.(i +^ 1us) n_threads_16 p)
-
-val put_thread (#o:_) (#p:tid -> vprop) (i:tid)
-  : STGhostT unit o
-    (p i `star`
-     forall_threads_between 0us i p `star`
-     forall_threads_between U16.(i +^ 1us) n_threads_16 p)
-    (fun _ -> forall_threads p)
-
-let refined_tid (p:tid -> Type0) = t:tid{p t}
-
-val update_forall_thread_between (#o:_)
-                                 (#p #q:tid -> vprop) (#refine:tid -> Type0)
-                                 (i:tid_index)
-                                 (j:tid_index{U16.v i <= U16.v j})
-                                 ($f: (k:refined_tid refine -> STGhostT unit o (p k) (fun _-> q k)))
-  : STGhost unit o
-     (forall_threads_between i j p)
-     (fun _ -> forall_threads_between i j q)
-     (requires (forall k. U16.v i <= U16.v k /\ U16.v k < U16.v j ==> refine k))
-     (ensures fun _ -> True)
-
+let hashes_bitmaps_max_ok (hashes:epoch_hashes_repr)
+                          (bitmaps: IArray.repr M.epoch_id tid_bitmap)
+                          (max:M.epoch_id)
+                          (mlogs_v:all_processed_entries)
+ : prop
+ = all_contributions_are_accurate hashes mlogs_v /\
+   max_certified_epoch_is hashes bitmaps max /\
+   (forall tid. per_thread_bitmap_and_max bitmaps max mlogs_v tid)
 
 let monotonic_logs = GMap.t tid log log_grows
 
@@ -232,8 +174,7 @@ let lock_inv_body (hashes : all_epoch_hashes)
     IArray.perm tid_bitmaps bitmaps Set.empty `star`
     R.pts_to max_certified_epoch full max `star`
     GMap.global_snapshot mlogs (map_of_seq mlogs_v) `star`
-    forall_threads (per_thread_invariant max bitmaps mlogs_v) `star`
-    pure (contribs_and_max_ok hashes_v bitmaps max mlogs_v)
+    pure (hashes_bitmaps_max_ok hashes_v bitmaps max mlogs_v)
 
 let lock_inv (hashes : all_epoch_hashes)
              (tid_bitmaps : epoch_tid_bitmaps)
@@ -256,18 +197,237 @@ type aggregate_epoch_hashes = {
      lock: cancellable_lock (lock_inv hashes tid_bitmaps max_certified_epoch mlogs)
 }
 
-let all_threads_have_processed (mlogs:monotonic_logs) (logs:all_processed_entries)
-  : vprop
-  = GMap.global_snapshot mlogs (map_of_seq logs)
+val check_bitmap_for_epoch (#bm:erased _)
+                           (tid_bitmaps: epoch_tid_bitmaps)
+                           (e:M.epoch_id)
+  : ST bool
+    (IArray.perm tid_bitmaps bm Set.empty)
+    (fun b -> IArray.perm tid_bitmaps bm Set.empty)
+    (requires True)
+    (ensures fun b -> b ==> Map.sel bm e == all_ones)
 
-let max_certified_epoch (logs:erased all_processed_entries)
-                        (aeh:aggregate_epoch_hashes)
-  : ST M.epoch_id
-      (all_threads_have_processed aeh.mlogs logs)
-      (fun _ -> all_threads_have_processed aeh.mlogs logs)
-      (requires True)
-      (ensures fun max ->
-            forall (eid:M.epoch_id).
-              U32.v eid <= U32.v max ==>
-              M.epoch_is_certified logs eid)
-  = admit__()
+val check_hash_equality_for_epoch (#hashes_v:erased _)
+                                  (hashes:all_epoch_hashes)
+                                  (e:M.epoch_id)
+  : ST bool
+    (IArray.perm hashes hashes_v Set.empty)
+    (fun _ -> IArray.perm hashes hashes_v Set.empty)
+    (requires True)
+    (ensures fun b ->
+      let ha = Map.sel hashes_v e in
+      b ==> ha.hadd == ha.hevict)
+
+let epoch_ready_if_bitmap_set (hashes:_)
+                              (bitmaps:_)
+                              (max:_)
+                              (mlogs_v:_)
+                              (e:M.epoch_id)
+  : Lemma
+    (requires
+      hashes_bitmaps_max_ok hashes bitmaps max mlogs_v /\
+      Map.sel bitmaps e == all_ones)
+    (ensures
+      epoch_is_complete mlogs_v e /\
+      Map.sel hashes e == aggregate_all_threads_epoch_hashes e mlogs_v)
+  = ()
+
+let epoch_is_certified (mlogs_v:all_processed_entries)
+                       (e:M.epoch_id)
+  = let hashes = aggregate_all_threads_epoch_hashes e mlogs_v in
+    epoch_is_complete mlogs_v e /\
+    hashes.hadd == hashes.hevict
+
+let max_is_correct (mlogs_v:_) (max:_)
+  : prop
+  = forall (e:M.epoch_id).
+          U32.v e <= U32.v max ==>
+          epoch_is_certified mlogs_v e
+
+let _max_is_correct (hashes:_)
+                    (bitmaps:_)
+                    (max:_)
+                    (mlogs_v:_)
+  : Lemma
+    (requires hashes_bitmaps_max_ok hashes bitmaps max mlogs_v)
+    (ensures  max_is_correct mlogs_v max)
+  = ()
+
+
+let try_increment_max (#hashes_v:erased _)
+                      (#bitmaps_v:erased _)
+                      (#mlogs_v:erased _)
+                      (hashes: all_epoch_hashes)
+                      (bitmaps: epoch_tid_bitmaps)
+                      (max:R.ref M.epoch_id)
+  : STT bool
+    (IArray.perm hashes hashes_v Set.empty `star`
+     IArray.perm bitmaps bitmaps_v Set.empty `star`
+     exists_ (fun max_v ->
+       R.pts_to max full max_v `star`
+       pure (hashes_bitmaps_max_ok hashes_v bitmaps_v max_v mlogs_v)))
+    (fun b ->
+      IArray.perm hashes hashes_v Set.empty `star`
+      IArray.perm bitmaps bitmaps_v Set.empty `star`
+      exists_ (fun (max_v':M.epoch_id) ->
+        R.pts_to max full max_v' `star`
+        pure (hashes_bitmaps_max_ok hashes_v bitmaps_v max_v' mlogs_v)))
+  = let max_v = elim_exists () in
+    let e = R.read max in
+    let v = check_overflow_add32 e 1ul in
+    match v with
+    | None ->
+      intro_exists_erased max_v (fun max_v' ->
+        R.pts_to max full max_v' `star`
+        pure (hashes_bitmaps_max_ok hashes_v bitmaps_v max_v' mlogs_v));
+      return false
+
+    | Some e' ->
+      let ready = check_bitmap_for_epoch bitmaps e' in
+      if not ready
+      then (
+        intro_exists_erased max_v (fun max_v' ->
+          R.pts_to max full max_v' `star`
+          pure (hashes_bitmaps_max_ok hashes_v bitmaps_v max_v' mlogs_v));
+        return false
+      )
+      else (
+        let b = check_hash_equality_for_epoch hashes e' in
+        if not b
+        then (
+          intro_exists_erased max_v (fun max_v' ->
+            R.pts_to max full max_v' `star`
+            pure (hashes_bitmaps_max_ok hashes_v bitmaps_v max_v' mlogs_v));
+          return false
+        )
+        else (
+          R.write max e';
+          elim_pure _;
+          intro_pure (hashes_bitmaps_max_ok hashes_v bitmaps_v e' mlogs_v);
+          intro_exists e' (fun max_v' ->
+            R.pts_to max full max_v' `star`
+            pure (hashes_bitmaps_max_ok hashes_v bitmaps_v max_v' mlogs_v));
+          return true
+        )
+      )
+
+val repeat_until (p: bool -> vprop)
+                 ($body: (unit -> STT bool (p true) (fun b -> p b)))
+  : STT unit (p true) (fun _ -> p false)
+
+let try_advance_max (#hashes_v:erased _)
+                    (#bitmaps_v:erased _)
+                    (#max_v:erased _)
+                    (#mlogs_v:erased _)
+                    (hashes: all_epoch_hashes)
+                    (bitmaps: epoch_tid_bitmaps)
+                    (max:R.ref M.epoch_id)
+  : STT M.epoch_id
+    (IArray.perm hashes hashes_v Set.empty `star`
+     IArray.perm bitmaps bitmaps_v Set.empty `star`
+     R.pts_to max full max_v `star`
+     pure (hashes_bitmaps_max_ok hashes_v bitmaps_v max_v mlogs_v))
+    (fun max_v' ->
+      IArray.perm hashes hashes_v Set.empty `star`
+      IArray.perm bitmaps bitmaps_v Set.empty `star`
+      R.pts_to max full max_v' `star`
+      pure (hashes_bitmaps_max_ok hashes_v bitmaps_v max_v' mlogs_v))
+  = intro_exists_erased max_v (fun max_v ->
+       R.pts_to max full max_v `star`
+       pure (hashes_bitmaps_max_ok hashes_v bitmaps_v max_v mlogs_v));
+    repeat_until _ (fun _ -> try_increment_max #hashes_v #bitmaps_v #mlogs_v hashes bitmaps max);
+    let _ = elim_exists _ in
+    let max = R.read max in
+    elim_pure _;
+    intro_pure _;
+    return max
+
+let release_lock (#hv:erased _)
+                 (#bitmaps:erased _)
+                 (#max:erased _)
+                 (#mlogs_v:erased _)
+                 (#hashes : all_epoch_hashes)
+                 (#tid_bitmaps : epoch_tid_bitmaps)
+                 (#max_certified_epoch : R.ref M.epoch_id)
+                 (#mlogs: monotonic_logs)
+                 (lock: cancellable_lock
+                        (lock_inv hashes tid_bitmaps max_certified_epoch mlogs))
+  : STT unit
+    (lock_inv_body hashes tid_bitmaps max_certified_epoch mlogs
+                       hv bitmaps max mlogs_v `star`
+     can_release lock)
+    (fun _ -> emp)
+  = intro_exists_erased mlogs_v
+      (fun mlogs_v ->  lock_inv_body hashes tid_bitmaps max_certified_epoch mlogs
+                                      hv bitmaps max mlogs_v);
+    intro_exists_erased max
+      (fun max ->
+        exists_ (fun mlogs_v ->
+                    lock_inv_body hashes tid_bitmaps max_certified_epoch mlogs
+                                      hv bitmaps max mlogs_v));
+    intro_exists_erased bitmaps
+      (fun bitmaps ->
+        exists_ (fun max ->
+        exists_ (fun mlogs_v ->
+                    lock_inv_body hashes tid_bitmaps max_certified_epoch mlogs
+                                      hv bitmaps max mlogs_v)));
+    intro_exists_erased hv
+      (fun hv ->
+        exists_ (fun bitmaps ->
+        exists_ (fun max ->
+        exists_ (fun mlogs_v ->
+                    lock_inv_body hashes tid_bitmaps max_certified_epoch mlogs
+                                      hv bitmaps max mlogs_v))));
+    release lock
+
+let advance_and_read_max_certified_epoch (aeh:aggregate_epoch_hashes)
+  : STT (option M.epoch_id)
+      emp
+      (fun max_opt ->
+        match max_opt with
+        | None -> emp //underspec: overflow or element went missing in IArray
+        | Some max ->
+          exists_ (fun logs ->
+           GMap.global_snapshot aeh.mlogs (map_of_seq logs) `star`
+           pure (max_is_correct logs max)))
+  = let b = acquire aeh.lock in
+    if not b
+    then (
+      rewrite (maybe_acquired _ _)
+              emp;
+      return None
+    )
+    else (
+      rewrite (maybe_acquired _ _)
+              (lock_inv aeh.hashes
+                        aeh.tid_bitmaps
+                        aeh.max_certified_epoch
+                        aeh.mlogs `star`
+              can_release aeh.lock);
+      let _hv = elim_exists () in
+      let _bitmaps = elim_exists () in
+      let _max = elim_exists () in
+      let _mlogs_v =
+          elim_exists #_ #_
+            #(lock_inv_body
+                 aeh.hashes
+                 aeh.tid_bitmaps
+                 aeh.max_certified_epoch
+                 aeh.mlogs
+                 _hv
+                 _bitmaps
+                 _max)
+            ()
+      in
+      let max = try_advance_max aeh.hashes aeh.tid_bitmaps aeh.max_certified_epoch in
+      extract_pure _;
+
+      intro_pure (max_is_correct _mlogs_v max);
+
+      GMap.dup_global_snapshot aeh.mlogs;
+      intro_exists_erased _mlogs_v
+        (fun logs ->
+           GMap.global_snapshot aeh.mlogs (map_of_seq logs) `star`
+           pure (max_is_correct logs max));
+      release_lock #_ #_ #(hide max) aeh.lock;
+      return (Some max)
+    )
